examples/dll_append.v
@@ -1,0 +1,242 @@
+From mathcomp
+Require Import ssreflect ssrbool ssrnat eqtype seq ssrfun.
+From fcsl
+Require Import prelude pred pcm unionmap heap.
+From HTT
+Require Import stmod stsep stlog stlogR.
+From SSL
+Require Import core.
+
+Inductive dll (x : ptr) (z : ptr) (s : seq nat) (h : heap) : Prop :=
+| dll_1 of x == null of
+  @perm_eq nat_eqType (s) (nil) /\ h = empty
+| dll_2 of (x == null) = false of
+  exists (v : nat) (s1 : seq nat) (w : ptr),
+  exists h_dll_wxs1_528,
+  @perm_eq nat_eqType (s) ([:: v] ++ s1) /\ h = x :-> v \+ x .+ 1 :-> w \+ x .+ 2 :-> z \+ h_dll_wxs1_528 /\ dll w x s1 h_dll_wxs1_528.
+
+Inductive sll (x : ptr) (s : seq nat) (h : heap) : Prop :=
+| sll_1 of x == null of
+  @perm_eq nat_eqType (s) (nil) /\ h = empty
+| sll_2 of (x == null) = false of
+  exists (v : nat) (s1 : seq nat) (nxt : ptr),
+  exists h_sll_nxts1_529,
+  @perm_eq nat_eqType (s) ([:: v] ++ s1) /\ h = x :-> v \+ x .+ 1 :-> nxt \+ h_sll_nxts1_529 /\ sll nxt s1 h_sll_nxts1_529.
+
+Lemma dll_perm_eq_trans19 x z h s_1 s_2 : perm_eq s_1 s_2 -> dll x z s_1 h -> dll x z s_2 h. Admitted.
+Hint Resolve dll_perm_eq_trans19: ssl_pred.
+Lemma sll_perm_eq_trans20 x h s_1 s_2 : perm_eq s_1 s_2 -> sll x s_1 h -> sll x s_2 h. Admitted.
+Hint Resolve sll_perm_eq_trans20: ssl_pred.
+Lemma pure21 vx12 s1x1 s2 : @perm_eq nat_eqType (s1x1 ++ s2) (nil) -> @perm_eq nat_eqType ([:: vx12] ++ s1x1 ++ s2) ([:: vx12]). Admitted.
+Hint Resolve pure21: ssl_pure.
+Lemma pure22 s2 s1x1 s1y12 vy122 vx12 : @perm_eq nat_eqType (s1x1 ++ s2) ([:: vy122] ++ s1y12) -> @perm_eq nat_eqType ([:: vx12] ++ s1x1 ++ s2) ([:: vx12] ++ [:: vy122] ++ s1y12). Admitted.
+Hint Resolve pure22: ssl_pure.
+
+Definition dll_append_type :=
+  forall (vprogs : ptr * ptr),
+  {(vghosts : ptr * seq nat * ptr * ptr * seq nat)},
+  STsep (
+    fun h =>
+      let: (x1, r) := vprogs in
+      let: (a, s1, x2, b, s2) := vghosts in
+      exists h_dll_x1as1_530 h_dll_x2bs2_531,
+      h = r :-> x2 \+ h_dll_x1as1_530 \+ h_dll_x2bs2_531 /\ dll x1 a s1 h_dll_x1as1_530 /\ dll x2 b s2 h_dll_x2bs2_531,
+    [vfun (_: unit) h =>
+      let: (x1, r) := vprogs in
+      let: (a, s1, x2, b, s2) := vghosts in
+      exists s y c,
+      exists h_dll_ycs_532,
+      @perm_eq nat_eqType (s) (s1 ++ s2) /\ h = r :-> y \+ h_dll_ycs_532 /\ dll y c s h_dll_ycs_532
+    ]).
+
+Program Definition dll_append : dll_append_type :=
+  Fix (fun (dll_append : dll_append_type) vprogs =>
+    let: (x1, r) := vprogs in
+    Do (
+      x22 <-- @read ptr r;
+      if x1 == null
+      then
+        ret tt
+      else
+        vx12 <-- @read nat x1;
+        wx12 <-- @read ptr (x1 .+ 1);
+        a2 <-- @read ptr (x1 .+ 2);
+        dll_append (wx12, r);;
+        y12 <-- @read ptr r;
+        if y12 == null
+        then
+          (x1 .+ 1) ::= null;;
+          r ::= x1;;
+          ret tt
+        else
+          vy122 <-- @read nat y12;
+          wy122 <-- @read ptr (y12 .+ 1);
+          c12 <-- @read ptr (y12 .+ 2);
+          (y12 .+ 2) ::= x1;;
+          (x1 .+ 1) ::= y12;;
+          r ::= x1;;
+          ret tt
+    )).
+Obligation Tactic := intro; move=>[x1 r]; ssl_program_simpl.
+Next Obligation.
+ssl_ghostelim_pre.
+move=>[[[[a s1] x2] b] s2].
+ex_elim h_dll_x1as1_530 h_dll_x2bs2_531.
+move=>[sigma_self].
+subst h_self.
+move=>[H_dll_x1as1_530 H_dll_x2bs2_531].
+ssl_ghostelim_post.
+try rename h_dll_ycs_532 into h_dll_ycs1s2_532.
+try rename H_dll_ycs_532 into H_dll_ycs1s2_532.
+ssl_read r.
+try rename x2 into x22.
+try rename h_dll_x2bs2_531 into h_dll_x22bs2_531.
+try rename H_dll_x2bs2_531 into H_dll_x22bs2_531.
+ssl_open (x1 == null) H_dll_x1as1_530.
+move=>[phi_dll_x1as1_5300].
+move=>[sigma_dll_x1as1_530].
+subst h_dll_x1as1_530.
+shelve.
+ex_elim vx1 s1x1 wx1.
+ex_elim h_dll_wx1x1s1x1_528x1.
+move=>[phi_dll_x1as1_5300].
+move=>[sigma_dll_x1as1_530].
+subst h_dll_x1as1_530.
+move=>H_dll_wx1x1s1x1_528x1.
+shelve.
+Unshelve.
+try rename h_dll_x1as1_530 into h_dll_x1a_530.
+try rename H_dll_x1as1_530 into H_dll_x1a_530.
+try rename h_dll_ycs1s2_532 into h_dll_ycs2_532.
+try rename H_dll_ycs1s2_532 into H_dll_ycs2_532.
+try rename h_dll_ycs2_532 into h_dll_ycs2_531.
+try rename H_dll_ycs2_532 into H_dll_ycs2_531.
+try rename h_dll_ycs2_531 into h_dll_ybs2_531.
+try rename H_dll_ycs2_531 into H_dll_ybs2_531.
+try rename h_dll_ybs2_531 into h_dll_x22bs2_531.
+try rename H_dll_ybs2_531 into H_dll_x22bs2_531.
+ssl_emp;
+exists (nil ++ s2), (x22), (b);
+exists (h_dll_x22bs2_531);
+sslauto.
+try rename h_dll_x1as1_530 into h_dll_x1avx1s1x1_530.
+try rename H_dll_x1as1_530 into H_dll_x1avx1s1x1_530.
+try rename h_dll_ycs1s2_532 into h_dll_ycvx1s1x1s2_532.
+try rename H_dll_ycs1s2_532 into H_dll_ycvx1s1x1s2_532.
+ssl_read x1.
+try rename vx1 into vx12.
+try rename h_dll_ycvx1s1x1s2_532 into h_dll_ycvx12s1x1s2_532.
+try rename H_dll_ycvx1s1x1s2_532 into H_dll_ycvx12s1x1s2_532.
+try rename h_dll_x1avx1s1x1_530 into h_dll_x1avx12s1x1_530.
+try rename H_dll_x1avx1s1x1_530 into H_dll_x1avx12s1x1_530.
+ssl_read (x1 .+ 1).
+try rename wx1 into wx12.
+try rename h_dll_wx1x1s1x1_528x1 into h_dll_wx12x1s1x1_528x1.
+try rename H_dll_wx1x1s1x1_528x1 into H_dll_wx12x1s1x1_528x1.
+ssl_read (x1 .+ 2).
+try rename a into a2.
+try rename h_dll_x1avx12s1x1_530 into h_dll_x1a2vx12s1x1_530.
+try rename H_dll_x1avx12s1x1_530 into H_dll_x1a2vx12s1x1_530.
+ssl_call_pre (r :-> x22 \+ h_dll_wx12x1s1x1_528x1 \+ h_dll_x22bs2_531).
+ssl_call (x1, s1x1, x22, b, s2).
+exists (h_dll_wx12x1s1x1_528x1), (h_dll_x22bs2_531);
+sslauto.
+move=>h_call0.
+ex_elim s3 y1 c1.
+ex_elim h_dll_y1c1s3_5321.
+move=>[phi_call00].
+move=>[sigma_call0].
+subst h_call0.
+move=>H_dll_y1c1s3_5321.
+store_valid.
+try rename h_dll_y1c1s3_5321 into h_dll_y1c1s1x1s2_5321.
+try rename H_dll_y1c1s3_5321 into H_dll_y1c1s1x1s2_5321.
+ssl_read r.
+try rename y1 into y12.
+try rename h_dll_y1c1s1x1s2_5321 into h_dll_y12c1s1x1s2_5321.
+try rename H_dll_y1c1s1x1s2_5321 into H_dll_y12c1s1x1s2_5321.
+ssl_open (y12 == null) H_dll_y12c1s1x1s2_5321.
+move=>[phi_dll_y12c1s1x1s2_53210].
+move=>[sigma_dll_y12c1s1x1s2_5321].
+subst h_dll_y12c1s1x1s2_5321.
+shelve.
+ex_elim vy12 s1y12 wy12.
+ex_elim h_dll_wy12y12s1y12_528y12.
+move=>[phi_dll_y12c1s1x1s2_53210].
+move=>[sigma_dll_y12c1s1x1s2_5321].
+subst h_dll_y12c1s1x1s2_5321.
+move=>H_dll_wy12y12s1y12_528y12.
+shelve.
+Unshelve.
+try rename h_dll_wyys12y_528y into h_dll_wyy_528y.
+try rename H_dll_wyys12y_528y into H_dll_wyy_528y.
+try rename h_dll_wyy_528y into h_dll_y_528y.
+try rename H_dll_wyy_528y into H_dll_y_528y.
+try rename h_dll_ycvx12s1x1s2_532 into h_dll_x1cvx12s1x1s2_532.
+try rename H_dll_ycvx12s1x1s2_532 into H_dll_x1cvx12s1x1s2_532.
+try rename h_dll_y_528y into h_dll_x1_528y.
+try rename H_dll_y_528y into H_dll_x1_528y.
+ssl_write (x1 .+ 1).
+ssl_write_post (x1 .+ 1).
+ssl_write r.
+ssl_write_post r.
+try rename h_dll_x1cvx12s1x1s2_532 into h_dll_x1a2vx12s1x1s2_532.
+try rename H_dll_x1cvx12s1x1s2_532 into H_dll_x1a2vx12s1x1s2_532.
+ssl_emp;
+exists ([:: vx12] ++ s1x1 ++ s2), (x1), (a2);
+exists (x1 :-> vx12 \+ x1 .+ 1 :-> null \+ x1 .+ 2 :-> a2);
+sslauto.
+unfold_constructor 2;
+exists (vx12), (nil), (null), (empty);
+sslauto.
+unfold_constructor 1;
+sslauto.
+ssl_read y12.
+try rename vy12 into vy122.
+ssl_read (y12 .+ 1).
+try rename wy12 into wy122.
+try rename h_dll_wy12y12s1y12_528y12 into h_dll_wy122y12s1y12_528y12.
+try rename H_dll_wy12y12s1y12_528y12 into H_dll_wy122y12s1y12_528y12.
+ssl_read (y12 .+ 2).
+try rename c1 into c12.
+try rename h_dll_y12c1s1x1s2_5321 into h_dll_y12c12s1x1s2_5321.
+try rename H_dll_y12c1s1x1s2_5321 into H_dll_y12c12s1x1s2_5321.
+try rename h_dll_wyys12y_528y into h_dll_wyyvwys12wy_528y.
+try rename H_dll_wyys12y_528y into H_dll_wyyvwys12wy_528y.
+try rename h_dll_wwywys12wy_528wy into h_dll_wwywys12wy_528y12.
+try rename H_dll_wwywys12wy_528wy into H_dll_wwywys12wy_528y12.
+try rename h_dll_wwywys12wy_528y12 into h_dll_wwywys1y12_528y12.
+try rename H_dll_wwywys12wy_528y12 into H_dll_wwywys1y12_528y12.
+try rename h_dll_wyyvwys12wy_528y into h_dll_wyyvwys1y12_528y.
+try rename H_dll_wyyvwys12wy_528y into H_dll_wyyvwys1y12_528y.
+try rename h_dll_wwywys1y12_528y12 into h_dll_wy122wys1y12_528y12.
+try rename H_dll_wwywys1y12_528y12 into H_dll_wy122wys1y12_528y12.
+try rename h_dll_wy122wys1y12_528y12 into h_dll_wy122y12s1y12_528y12.
+try rename H_dll_wy122wys1y12_528y12 into H_dll_wy122y12s1y12_528y12.
+try rename h_dll_wyyvwys1y12_528y into h_dll_y12yvwys1y12_528y.
+try rename H_dll_wyyvwys1y12_528y into H_dll_y12yvwys1y12_528y.
+try rename h_dll_ycvx12s1x1s2_532 into h_dll_x1cvx12s1x1s2_532.
+try rename H_dll_ycvx12s1x1s2_532 into H_dll_x1cvx12s1x1s2_532.
+try rename h_dll_y12yvwys1y12_528y into h_dll_y12x1vwys1y12_528y.
+try rename H_dll_y12yvwys1y12_528y into H_dll_y12x1vwys1y12_528y.
+ssl_write (y12 .+ 2).
+ssl_write_post (y12 .+ 2).
+ssl_write (x1 .+ 1).
+ssl_write_post (x1 .+ 1).
+ssl_write r.
+ssl_write_post r.
+try rename h_dll_x1cvx12s1x1s2_532 into h_dll_x1a2vx12s1x1s2_532.
+try rename H_dll_x1cvx12s1x1s2_532 into H_dll_x1a2vx12s1x1s2_532.
+try rename h_dll_y12x1vwys1y12_528y into h_dll_y12x1vy122s1y12_528y.
+try rename H_dll_y12x1vwys1y12_528y into H_dll_y12x1vy122s1y12_528y.
+ssl_emp;
+exists ([:: vx12] ++ s1x1 ++ s2), (x1), (a2);
+exists (x1 :-> vx12 \+ x1 .+ 1 :-> y12 \+ x1 .+ 2 :-> a2 \+ y12 :-> vy122 \+ y12 .+ 1 :-> wy122 \+ y12 .+ 2 :-> x1 \+ h_dll_wy122y12s1y12_528y12);
+sslauto.
+unfold_constructor 2;
+exists (vx12), ([:: vy122] ++ s1y12), (y12), (y12 :-> vy122 \+ y12 .+ 1 :-> wy122 \+ y12 .+ 2 :-> x1 \+ h_dll_wy122y12s1y12_528y12);
+sslauto.
+unfold_constructor 2;
+exists (vy122), (s1y12), (wy122), (h_dll_wy122y12s1y12_528y12);
+sslauto.
+Qed.
