examples/dll_copy.v
@@ -1,0 +1,333 @@
+From mathcomp
+Require Import ssreflect ssrbool ssrnat eqtype seq ssrfun.
+From fcsl
+Require Import prelude pred pcm unionmap heap.
+From HTT
+Require Import stmod stsep stlog stlogR.
+From SSL
+Require Import core.
+
+Inductive dll (x : ptr) (z : ptr) (s : seq nat) (h : heap) : Prop :=
+| dll_1 of x == null of
+  @perm_eq nat_eqType (s) (nil) /\ h = empty
+| dll_2 of (x == null) = false of
+  exists (v : nat) (s1 : seq nat) (w : ptr),
+  exists h_dll_wxs1_513,
+  @perm_eq nat_eqType (s) ([:: v] ++ s1) /\ h = x :-> v \+ x .+ 1 :-> w \+ x .+ 2 :-> z \+ h_dll_wxs1_513 /\ dll w x s1 h_dll_wxs1_513.
+
+Inductive sll (x : ptr) (s : seq nat) (h : heap) : Prop :=
+| sll_1 of x == null of
+  @perm_eq nat_eqType (s) (nil) /\ h = empty
+| sll_2 of (x == null) = false of
+  exists (v : nat) (s1 : seq nat) (nxt : ptr),
+  exists h_sll_nxts1_514,
+  @perm_eq nat_eqType (s) ([:: v] ++ s1) /\ h = x :-> v \+ x .+ 1 :-> nxt \+ h_sll_nxts1_514 /\ sll nxt s1 h_sll_nxts1_514.
+
+Lemma dll_perm_eq_trans1 x z h s_1 s_2 : perm_eq s_1 s_2 -> dll x z s_1 h -> dll x z s_2 h. Admitted.
+Hint Resolve dll_perm_eq_trans1: ssl_pred.
+Lemma sll_perm_eq_trans2 x h s_1 s_2 : perm_eq s_1 s_2 -> sll x s_1 h -> sll x s_2 h. Admitted.
+Hint Resolve sll_perm_eq_trans2: ssl_pred.
+Lemma pure3 : @perm_eq nat_eqType (nil) (nil). Admitted.
+Hint Resolve pure3: ssl_pure.
+Lemma pure4 vx22 : @perm_eq nat_eqType ([:: vx22]) ([:: vx22]). Admitted.
+Hint Resolve pure4: ssl_pure.
+Lemma pure5 vx22 : @perm_eq nat_eqType ([:: vx22]) ([:: vx22]). Admitted.
+Hint Resolve pure5: ssl_pure.
+Lemma pure6 vx22 vy122 s1y12 : @perm_eq nat_eqType ([:: vx22] ++ [:: vy122] ++ s1y12) ([:: vx22] ++ [:: vy122] ++ s1y12). Admitted.
+Hint Resolve pure6: ssl_pure.
+Lemma pure7 vx22 vy122 s1y12 : @perm_eq nat_eqType ([:: vx22] ++ [:: vy122] ++ s1y12) ([:: vy122] ++ [:: vx22] ++ s1y12). Admitted.
+Hint Resolve pure7: ssl_pure.
+
+Definition dll_copy_type :=
+  forall (vprogs : ptr),
+  {(vghosts : ptr * ptr * seq nat)},
+  STsep (
+    fun h =>
+      let: (r) := vprogs in
+      let: (x, a, s) := vghosts in
+      exists h_dll_xas_515,
+      h = r :-> x \+ h_dll_xas_515 /\ dll x a s h_dll_xas_515,
+    [vfun (_: unit) h =>
+      let: (r) := vprogs in
+      let: (x, a, s) := vghosts in
+      exists y b,
+      exists h_dll_xas_516 h_dll_ybs_517,
+      h = r :-> y \+ h_dll_xas_516 \+ h_dll_ybs_517 /\ dll x a s h_dll_xas_516 /\ dll y b s h_dll_ybs_517
+    ]).
+
+Program Definition dll_copy : dll_copy_type :=
+  Fix (fun (dll_copy : dll_copy_type) vprogs =>
+    let: (r) := vprogs in
+    Do (
+      x2 <-- @read ptr r;
+      if x2 == null
+      then
+        ret tt
+      else
+        vx22 <-- @read nat x2;
+        wx22 <-- @read ptr (x2 .+ 1);
+        a2 <-- @read ptr (x2 .+ 2);
+        r ::= wx22;;
+        dll_copy (r);;
+        y12 <-- @read ptr r;
+        if y12 == null
+        then
+          y2 <-- allocb null 3;
+          r ::= y2;;
+          (y2 .+ 1) ::= null;;
+          y2 ::= vx22;;
+          (y2 .+ 2) ::= null;;
+          ret tt
+        else
+          vy122 <-- @read nat y12;
+          wy122 <-- @read ptr (y12 .+ 1);
+          b12 <-- @read ptr (y12 .+ 2);
+          y2 <-- allocb null 3;
+          (y12 .+ 2) ::= y2;;
+          r ::= y2;;
+          (y2 .+ 1) ::= y12;;
+          y12 ::= vx22;;
+          y2 ::= vy122;;
+          (y2 .+ 2) ::= null;;
+          ret tt
+    )).
+Obligation Tactic := intro; move=>r; ssl_program_simpl.
+Next Obligation.
+ssl_ghostelim_pre.
+move=>[[x a] s].
+ex_elim h_dll_xas_515.
+move=>[sigma_self].
+subst h_self.
+move=>H_dll_xas_515.
+ssl_ghostelim_post.
+ssl_read r.
+try rename x into x2.
+try rename h_dll_xas_515 into h_dll_x2as_515.
+try rename H_dll_xas_515 into H_dll_x2as_515.
+try rename h_dll_xas_516 into h_dll_x2as_516.
+try rename H_dll_xas_516 into H_dll_x2as_516.
+ssl_open (x2 == null) H_dll_x2as_515.
+move=>[phi_dll_x2as_5150].
+move=>[sigma_dll_x2as_515].
+subst h_dll_x2as_515.
+shelve.
+ex_elim vx2 s1x2 wx2.
+ex_elim h_dll_wx2x2s1x2_513x2.
+move=>[phi_dll_x2as_5150].
+move=>[sigma_dll_x2as_515].
+subst h_dll_x2as_515.
+move=>H_dll_wx2x2s1x2_513x2.
+shelve.
+Unshelve.
+try rename h_dll_x2as_515 into h_dll_x2a_515.
+try rename H_dll_x2as_515 into H_dll_x2a_515.
+try rename h_dll_ybs_517 into h_dll_yb_517.
+try rename H_dll_ybs_517 into H_dll_yb_517.
+try rename h_dll_x2as_516 into h_dll_x2a_516.
+try rename H_dll_x2as_516 into H_dll_x2a_516.
+try rename h_dll_yb_517 into h_dll_b_517.
+try rename H_dll_yb_517 into H_dll_b_517.
+ssl_emp;
+exists (null), (null);
+exists (empty);
+exists (empty);
+sslauto.
+unfold_constructor 1;
+sslauto.
+unfold_constructor 1;
+sslauto.
+try rename h_dll_x2as_515 into h_dll_x2avx2s1x2_515.
+try rename H_dll_x2as_515 into H_dll_x2avx2s1x2_515.
+try rename h_dll_ybs_517 into h_dll_ybvx2s1x2_517.
+try rename H_dll_ybs_517 into H_dll_ybvx2s1x2_517.
+try rename h_dll_x2as_516 into h_dll_x2avx2s1x2_516.
+try rename H_dll_x2as_516 into H_dll_x2avx2s1x2_516.
+ssl_read x2.
+try rename vx2 into vx22.
+try rename h_dll_x2avx2s1x2_516 into h_dll_x2avx22s1x2_516.
+try rename H_dll_x2avx2s1x2_516 into H_dll_x2avx22s1x2_516.
+try rename h_dll_x2avx2s1x2_515 into h_dll_x2avx22s1x2_515.
+try rename H_dll_x2avx2s1x2_515 into H_dll_x2avx22s1x2_515.
+try rename h_dll_ybvx2s1x2_517 into h_dll_ybvx22s1x2_517.
+try rename H_dll_ybvx2s1x2_517 into H_dll_ybvx22s1x2_517.
+ssl_read (x2 .+ 1).
+try rename wx2 into wx22.
+try rename h_dll_wx2x2s1x2_513x2 into h_dll_wx22x2s1x2_513x2.
+try rename H_dll_wx2x2s1x2_513x2 into H_dll_wx22x2s1x2_513x2.
+ssl_read (x2 .+ 2).
+try rename a into a2.
+try rename h_dll_x2avx22s1x2_515 into h_dll_x2a2vx22s1x2_515.
+try rename H_dll_x2avx22s1x2_515 into H_dll_x2a2vx22s1x2_515.
+try rename h_dll_x2avx22s1x2_516 into h_dll_x2a2vx22s1x2_516.
+try rename H_dll_x2avx22s1x2_516 into H_dll_x2a2vx22s1x2_516.
+ssl_write r.
+ssl_call_pre (r :-> wx22 \+ h_dll_wx22x2s1x2_513x2).
+ssl_call (wx22, x2, s1x2).
+exists (h_dll_wx22x2s1x2_513x2);
+sslauto.
+move=>h_call0.
+ex_elim y1 b1.
+ex_elim h_dll_wx22x2s1x2_5161 h_dll_y1b1s1x2_5171.
+move=>[sigma_call0].
+subst h_call0.
+move=>[H_dll_wx22x2s1x2_5161 H_dll_y1b1s1x2_5171].
+store_valid.
+ssl_read r.
+try rename y1 into y12.
+try rename h_dll_y1b1s1x2_5171 into h_dll_y12b1s1x2_5171.
+try rename H_dll_y1b1s1x2_5171 into H_dll_y12b1s1x2_5171.
+ssl_open (y12 == null) H_dll_y12b1s1x2_5171.
+move=>[phi_dll_y12b1s1x2_51710].
+move=>[sigma_dll_y12b1s1x2_5171].
+subst h_dll_y12b1s1x2_5171.
+shelve.
+ex_elim vy12 s1y12 wy12.
+ex_elim h_dll_wy12y12s1y12_513y12.
+move=>[phi_dll_y12b1s1x2_51710].
+move=>[sigma_dll_y12b1s1x2_5171].
+subst h_dll_y12b1s1x2_5171.
+move=>H_dll_wy12y12s1y12_513y12.
+shelve.
+Unshelve.
+try rename h_dll_y12b1s1x2_5171 into h_dll_y12b1_5171.
+try rename H_dll_y12b1s1x2_5171 into H_dll_y12b1_5171.
+try rename h_dll_x2a2vx22s1x2_515 into h_dll_x2a2vx22_515.
+try rename H_dll_x2a2vx22s1x2_515 into H_dll_x2a2vx22_515.
+try rename h_dll_wx22x2s1x2_513x2 into h_dll_wx22x2_513x2.
+try rename H_dll_wx22x2s1x2_513x2 into H_dll_wx22x2_513x2.
+try rename h_dll_ybvx22s1x2_517 into h_dll_ybvx22_517.
+try rename H_dll_ybvx22s1x2_517 into H_dll_ybvx22_517.
+try rename h_dll_x2a2vx22s1x2_516 into h_dll_x2a2vx22_516.
+try rename H_dll_x2a2vx22s1x2_516 into H_dll_x2a2vx22_516.
+try rename h_dll_wx22x2s1x2_5161 into h_dll_wx22x2_5161.
+try rename H_dll_wx22x2s1x2_5161 into H_dll_wx22x2_5161.
+try rename h_dll_wyys11y_513y into h_dll_wyy_513y.
+try rename H_dll_wyys11y_513y into H_dll_wyy_513y.
+try rename h_dll_wyy_513y into h_dll_y_513y.
+try rename H_dll_wyy_513y into H_dll_y_513y.
+try rename h_dll_wx21x2s11x2_513x21 into h_dll_wx21x2s11x2_5161.
+try rename H_dll_wx21x2s11x2_513x21 into H_dll_wx21x2s11x2_5161.
+try rename h_dll_wx21x2s11x2_5161 into h_dll_wx21x2_5161.
+try rename H_dll_wx21x2s11x2_5161 into H_dll_wx21x2_5161.
+try rename h_dll_wx21x2_5161 into h_dll_wx22x2_5161.
+try rename H_dll_wx21x2_5161 into H_dll_wx22x2_5161.
+ssl_alloc y2.
+try rename y into y2.
+try rename h_dll_y_513y into h_dll_y2_513y.
+try rename H_dll_y_513y into H_dll_y2_513y.
+try rename h_dll_ybvx22_517 into h_dll_y2bvx22_517.
+try rename H_dll_ybvx22_517 into H_dll_y2bvx22_517.
+ssl_write r.
+ssl_write_post r.
+ssl_write (y2 .+ 1).
+ssl_write_post (y2 .+ 1).
+try rename h_dll_y2bvx22_517 into h_dll_y2vx22_517.
+try rename H_dll_y2bvx22_517 into H_dll_y2vx22_517.
+ssl_write y2.
+ssl_write_post y2.
+ssl_write (y2 .+ 2).
+ssl_write_post (y2 .+ 2).
+ssl_emp;
+exists (y2), (null);
+exists (x2 :-> vx22 \+ x2 .+ 1 :-> wx22 \+ x2 .+ 2 :-> a2 \+ h_dll_wx22x2_5161);
+exists (y2 :-> vx22 \+ y2 .+ 1 :-> null \+ y2 .+ 2 :-> null);
+sslauto.
+unfold_constructor 2;
+exists (vx22), (nil), (wx22), (h_dll_wx22x2_5161);
+sslauto.
+unfold_constructor 2;
+exists (vx22), (nil), (null), (empty);
+sslauto.
+unfold_constructor 1;
+sslauto.
+try rename h_dll_y12b1s1x2_5171 into h_dll_y12b1vy12s1y12_5171.
+try rename H_dll_y12b1s1x2_5171 into H_dll_y12b1vy12s1y12_5171.
+try rename h_dll_x2a2vx22s1x2_515 into h_dll_x2a2vx22vy12s1y12_515.
+try rename H_dll_x2a2vx22s1x2_515 into H_dll_x2a2vx22vy12s1y12_515.
+try rename h_dll_wx22x2s1x2_513x2 into h_dll_wx22x2vy12s1y12_513x2.
+try rename H_dll_wx22x2s1x2_513x2 into H_dll_wx22x2vy12s1y12_513x2.
+try rename h_dll_ybvx22s1x2_517 into h_dll_ybvx22vy12s1y12_517.
+try rename H_dll_ybvx22s1x2_517 into H_dll_ybvx22vy12s1y12_517.
+try rename h_dll_x2a2vx22s1x2_516 into h_dll_x2a2vx22vy12s1y12_516.
+try rename H_dll_x2a2vx22s1x2_516 into H_dll_x2a2vx22vy12s1y12_516.
+try rename h_dll_wx22x2s1x2_5161 into h_dll_wx22x2vy12s1y12_5161.
+try rename H_dll_wx22x2s1x2_5161 into H_dll_wx22x2vy12s1y12_5161.
+ssl_read y12.
+try rename vy12 into vy122.
+try rename h_dll_x2a2vx22vy12s1y12_515 into h_dll_x2a2vx22vy122s1y12_515.
+try rename H_dll_x2a2vx22vy12s1y12_515 into H_dll_x2a2vx22vy122s1y12_515.
+try rename h_dll_x2a2vx22vy12s1y12_516 into h_dll_x2a2vx22vy122s1y12_516.
+try rename H_dll_x2a2vx22vy12s1y12_516 into H_dll_x2a2vx22vy122s1y12_516.
+try rename h_dll_wx22x2vy12s1y12_513x2 into h_dll_wx22x2vy122s1y12_513x2.
+try rename H_dll_wx22x2vy12s1y12_513x2 into H_dll_wx22x2vy122s1y12_513x2.
+try rename h_dll_ybvx22vy12s1y12_517 into h_dll_ybvx22vy122s1y12_517.
+try rename H_dll_ybvx22vy12s1y12_517 into H_dll_ybvx22vy122s1y12_517.
+try rename h_dll_y12b1vy12s1y12_5171 into h_dll_y12b1vy122s1y12_5171.
+try rename H_dll_y12b1vy12s1y12_5171 into H_dll_y12b1vy122s1y12_5171.
+try rename h_dll_wx22x2vy12s1y12_5161 into h_dll_wx22x2vy122s1y12_5161.
+try rename H_dll_wx22x2vy12s1y12_5161 into H_dll_wx22x2vy122s1y12_5161.
+ssl_read (y12 .+ 1).
+try rename wy12 into wy122.
+try rename h_dll_wy12y12s1y12_513y12 into h_dll_wy122y12s1y12_513y12.
+try rename H_dll_wy12y12s1y12_513y12 into H_dll_wy122y12s1y12_513y12.
+ssl_read (y12 .+ 2).
+try rename b1 into b12.
+try rename h_dll_y12b1vy122s1y12_5171 into h_dll_y12b12vy122s1y12_5171.
+try rename H_dll_y12b1vy122s1y12_5171 into H_dll_y12b12vy122s1y12_5171.
+try rename h_dll_wyys11y_513y into h_dll_wyyvwys11wy_513y.
+try rename H_dll_wyys11y_513y into H_dll_wyyvwys11wy_513y.
+try rename h_dll_wx21x2s11x2_513x21 into h_dll_wx21x2s11x2_5161.
+try rename H_dll_wx21x2s11x2_513x21 into H_dll_wx21x2s11x2_5161.
+try rename h_dll_wx21x2s11x2_5161 into h_dll_wx21x2vy122s1y12_5161.
+try rename H_dll_wx21x2s11x2_5161 into H_dll_wx21x2vy122s1y12_5161.
+try rename h_dll_wx21x2vy122s1y12_5161 into h_dll_wx22x2vy122s1y12_5161.
+try rename H_dll_wx21x2vy122s1y12_5161 into H_dll_wx22x2vy122s1y12_5161.
+try rename h_dll_wwywys11wy_513wy into h_dll_wwywys11wy_513y12.
+try rename H_dll_wwywys11wy_513wy into H_dll_wwywys11wy_513y12.
+try rename h_dll_wwywys11wy_513y12 into h_dll_wwywys1y12_513y12.
+try rename H_dll_wwywys11wy_513y12 into H_dll_wwywys1y12_513y12.
+try rename h_dll_wyyvwys11wy_513y into h_dll_wyyvwys1y12_513y.
+try rename H_dll_wyyvwys11wy_513y into H_dll_wyyvwys1y12_513y.
+try rename h_dll_wwywys1y12_513y12 into h_dll_wy122wys1y12_513y12.
+try rename H_dll_wwywys1y12_513y12 into H_dll_wy122wys1y12_513y12.
+try rename h_dll_wy122wys1y12_513y12 into h_dll_wy122y12s1y12_513y12.
+try rename H_dll_wy122wys1y12_513y12 into H_dll_wy122y12s1y12_513y12.
+try rename h_dll_wyyvwys1y12_513y into h_dll_y12yvwys1y12_513y.
+try rename H_dll_wyyvwys1y12_513y into H_dll_y12yvwys1y12_513y.
+ssl_alloc y2.
+try rename y into y2.
+try rename h_dll_y12yvwys1y12_513y into h_dll_y12y2vwys1y12_513y.
+try rename H_dll_y12yvwys1y12_513y into H_dll_y12y2vwys1y12_513y.
+try rename h_dll_ybvx22vy122s1y12_517 into h_dll_y2bvx22vy122s1y12_517.
+try rename H_dll_ybvx22vy122s1y12_517 into H_dll_y2bvx22vy122s1y12_517.
+ssl_write (y12 .+ 2).
+ssl_write_post (y12 .+ 2).
+ssl_write r.
+ssl_write_post r.
+ssl_write (y2 .+ 1).
+ssl_write_post (y2 .+ 1).
+try rename h_dll_y2bvx22vy122s1y12_517 into h_dll_y2vx22vy122s1y12_517.
+try rename H_dll_y2bvx22vy122s1y12_517 into H_dll_y2vx22vy122s1y12_517.
+try rename h_dll_y12y2vwys1y12_513y into h_dll_y12y2vx22s1y12_513y.
+try rename H_dll_y12y2vwys1y12_513y into H_dll_y12y2vx22s1y12_513y.
+ssl_write y12.
+ssl_write_post y12.
+ssl_write y2.
+ssl_write_post y2.
+ssl_write (y2 .+ 2).
+ssl_write_post (y2 .+ 2).
+ssl_emp;
+exists (y2), (null);
+exists (x2 :-> vx22 \+ x2 .+ 1 :-> wx22 \+ x2 .+ 2 :-> a2 \+ h_dll_wx22x2vy122s1y12_5161);
+exists (y2 :-> vy122 \+ y2 .+ 1 :-> y12 \+ y2 .+ 2 :-> null \+ y12 :-> vx22 \+ y12 .+ 1 :-> wy122 \+ y12 .+ 2 :-> y2 \+ h_dll_wy122y12s1y12_513y12);
+sslauto.
+unfold_constructor 2;
+exists (vx22), ([:: vy122] ++ s1y12), (wx22), (h_dll_wx22x2vy122s1y12_5161);
+sslauto.
+unfold_constructor 2;
+exists (vy122), ([:: vx22] ++ s1y12), (y12), (y12 :-> vx22 \+ y12 .+ 1 :-> wy122 \+ y12 .+ 2 :-> y2 \+ h_dll_wy122y12s1y12_513y12);
+sslauto.
+unfold_constructor 2;
+exists (vx22), (s1y12), (wy122), (h_dll_wy122y12s1y12_513y12);
+sslauto.
+Qed.
