examples/insertion_sort.v
@@ -1,0 +1,236 @@
+From mathcomp
+Require Import ssreflect ssrbool ssrnat eqtype seq ssrfun.
+From fcsl
+Require Import prelude pred pcm unionmap heap.
+From HTT
+Require Import stmod stsep stlog stlogR.
+From SSL
+Require Import core.
+
+Inductive sll (x : ptr) (len : nat) (lo : nat) (hi : nat) (h : heap) : Prop :=
+| sll_1 of x == null of
+  hi == 0 /\ len == 0 /\ lo == 7 /\ h = empty
+| sll_2 of (x == null) = false of
+  exists (len1 : nat) (v : nat) (hi1 : nat) (lo1 : nat) (nxt : ptr),
+  exists h_sll_nxtlen1lo1hi1_513,
+  0 <= len1 /\ 0 <= v /\ hi == (if hi1 <= v then v else hi1) /\ len == 1 + len1 /\ lo == (if v <= lo1 then v else lo1) /\ v <= 7 /\ h = x :-> v \+ x .+ 1 :-> nxt \+ h_sll_nxtlen1lo1hi1_513 /\ sll nxt len1 lo1 hi1 h_sll_nxtlen1lo1hi1_513.
+
+Inductive srtl (x : ptr) (len : nat) (lo : nat) (hi : nat) (h : heap) : Prop :=
+| srtl_1 of x == null of
+  hi == 0 /\ len == 0 /\ lo == 7 /\ h = empty
+| srtl_2 of (x == null) = false of
+  exists (len1 : nat) (v : nat) (hi1 : nat) (lo1 : nat) (nxt : ptr),
+  exists h_srtl_nxtlen1lo1hi1_514,
+  0 <= len1 /\ 0 <= v /\ hi == (if hi1 <= v then v else hi1) /\ len == 1 + len1 /\ lo == (if v <= lo1 then v else lo1) /\ v <= 7 /\ v <= lo1 /\ h = x :-> v \+ x .+ 1 :-> nxt \+ h_srtl_nxtlen1lo1hi1_514 /\ srtl nxt len1 lo1 hi1 h_srtl_nxtlen1lo1hi1_514.
+
+Lemma pure1 : 0 == 0. Admitted.
+Hint Resolve pure1: ssl_pure.
+Lemma pure2 : 7 == 7. Admitted.
+Hint Resolve pure2: ssl_pure.
+Lemma pure3 hi1x vx2 : 0 <= vx2 -> vx2 <= 7 -> (if hi1x <= vx2 then vx2 else hi1x) == (if hi1x <= vx2 then vx2 else hi1x). Admitted.
+Hint Resolve pure3: ssl_pure.
+Lemma pure4 len1x : 0 <= 1 + len1x -> 0 <= len1x -> 1 + len1x == 1 + len1x. Admitted.
+Hint Resolve pure4: ssl_pure.
+Lemma pure5 vx2 lo1x : 0 <= vx2 -> vx2 <= 7 -> (if vx2 <= lo1x then vx2 else lo1x) == (if vx2 <= lo1x then vx2 else lo1x). Admitted.
+Hint Resolve pure5: ssl_pure.
+Lemma pure6 hi1x vx2 : 0 <= vx2 -> vx2 <= 7 -> (if hi1x <= vx2 then vx2 else hi1x) == (if hi1x <= vx2 then vx2 else hi1x). Admitted.
+Hint Resolve pure6: ssl_pure.
+Lemma pure7 vx2 lo1x : 0 <= vx2 -> vx2 <= 7 -> (if vx2 <= lo1x then vx2 else lo1x) == (if vx2 <= lo1x then vx2 else lo1x). Admitted.
+Hint Resolve pure7: ssl_pure.
+
+Definition srtl_insert_type :=
+  forall (vprogs : ptr * ptr),
+  {(vghosts : nat * nat * nat * nat)},
+  STsep (
+    fun h =>
+      let: (x, r) := vprogs in
+      let: (k, n, lo, hi) := vghosts in
+      exists h_srtl_xnlohi_515,
+      0 <= k /\ 0 <= n /\ k <= 7 /\ h = r :-> k \+ h_srtl_xnlohi_515 /\ srtl x n lo hi h_srtl_xnlohi_515,
+    [vfun (_: unit) h =>
+      let: (x, r) := vprogs in
+      let: (k, n, lo, hi) := vghosts in
+      exists hi1 lo1 n1 y,
+      exists h_srtl_yn1lo1hi1_516,
+      hi1 == (if hi <= k then k else hi) /\ lo1 == (if k <= lo then k else lo) /\ n1 == 1 + n /\ h = r :-> y \+ h_srtl_yn1lo1hi1_516 /\ srtl y n1 lo1 hi1 h_srtl_yn1lo1hi1_516
+    ]).
+
+Variable srtl_insert : srtl_insert_type.
+
+Definition insertion_sort_type :=
+  forall (vprogs : ptr * ptr),
+  {(vghosts : nat * nat * nat)},
+  STsep (
+    fun h =>
+      let: (x, r) := vprogs in
+      let: (n, lo, hi) := vghosts in
+      exists h_sll_xnlohi_517,
+      0 <= n /\ h = r :-> null \+ h_sll_xnlohi_517 /\ sll x n lo hi h_sll_xnlohi_517,
+    [vfun (_: unit) h =>
+      let: (x, r) := vprogs in
+      let: (n, lo, hi) := vghosts in
+      exists y,
+      exists h_sll_xnlohi_518 h_srtl_ynlohi_519,
+      h = r :-> y \+ h_sll_xnlohi_518 \+ h_srtl_ynlohi_519 /\ sll x n lo hi h_sll_xnlohi_518 /\ srtl y n lo hi h_srtl_ynlohi_519
+    ]).
+
+Program Definition insertion_sort : insertion_sort_type :=
+  Fix (fun (insertion_sort : insertion_sort_type) vprogs =>
+    let: (x, r) := vprogs in
+    Do (
+      if x == null
+      then
+        ret tt
+      else
+        vx2 <-- @read nat x;
+        nxtx2 <-- @read ptr (x .+ 1);
+        insertion_sort (nxtx2, r);;
+        y12 <-- @read ptr r;
+        r ::= vx2;;
+        srtl_insert (y12, r);;
+        y22 <-- @read ptr r;
+        ret tt
+    )).
+Obligation Tactic := intro; move=>[x r]; ssl_program_simpl.
+Next Obligation.
+ssl_ghostelim_pre.
+move=>[[n lo] hi].
+ex_elim h_sll_xnlohi_517.
+move=>[phi_self0].
+move=>[sigma_self].
+subst h_self.
+move=>H_sll_xnlohi_517.
+ssl_ghostelim_post.
+ssl_open (x == null) H_sll_xnlohi_517.
+move=>[phi_sll_xnlohi_5170] [phi_sll_xnlohi_5171] [phi_sll_xnlohi_5172].
+move=>[sigma_sll_xnlohi_517].
+subst h_sll_xnlohi_517.
+shelve.
+ex_elim len1x vx hi1x lo1x nxtx.
+ex_elim h_sll_nxtxlen1xlo1xhi1x_513x.
+move=>[phi_sll_xnlohi_5170] [phi_sll_xnlohi_5171] [phi_sll_xnlohi_5172] [phi_sll_xnlohi_5173] [phi_sll_xnlohi_5174] [phi_sll_xnlohi_5175].
+move=>[sigma_sll_xnlohi_517].
+subst h_sll_xnlohi_517.
+move=>H_sll_nxtxlen1xlo1xhi1x_513x.
+shelve.
+Unshelve.
+try rename h_sll_xnlohi_517 into h_sll_xnlo_517.
+try rename H_sll_xnlohi_517 into H_sll_xnlo_517.
+try rename h_sll_xnlohi_518 into h_sll_xnlo_518.
+try rename H_sll_xnlohi_518 into H_sll_xnlo_518.
+try rename h_srtl_ynlohi_519 into h_srtl_ynlo_519.
+try rename H_srtl_ynlohi_519 into H_srtl_ynlo_519.
+try rename h_srtl_ynlo_519 into h_srtl_yn_519.
+try rename H_srtl_ynlo_519 into H_srtl_yn_519.
+try rename h_sll_xnlo_518 into h_sll_xn_518.
+try rename H_sll_xnlo_518 into H_sll_xn_518.
+try rename h_sll_xnlo_517 into h_sll_xn_517.
+try rename H_sll_xnlo_517 into H_sll_xn_517.
+try rename h_sll_xn_517 into h_sll_x_517.
+try rename H_sll_xn_517 into H_sll_x_517.
+try rename h_srtl_yn_519 into h_srtl_y_519.
+try rename H_srtl_yn_519 into H_srtl_y_519.
+try rename h_sll_xn_518 into h_sll_x_518.
+try rename H_sll_xn_518 into H_sll_x_518.
+try rename h_srtl_y_519 into h_srtl__519.
+try rename H_srtl_y_519 into H_srtl__519.
+ssl_emp;
+exists (null);
+exists (empty);
+exists (empty);
+sslauto.
+unfold_constructor 1;
+sslauto.
+unfold_constructor 1;
+sslauto.
+try rename h_sll_xnlohi_517 into h_sll_xnlohi1xvxvxhi1x_517.
+try rename H_sll_xnlohi_517 into H_sll_xnlohi1xvxvxhi1x_517.
+try rename h_sll_xnlohi_518 into h_sll_xnlohi1xvxvxhi1x_518.
+try rename H_sll_xnlohi_518 into H_sll_xnlohi1xvxvxhi1x_518.
+try rename h_srtl_ynlohi_519 into h_srtl_ynlohi1xvxvxhi1x_519.
+try rename H_srtl_ynlohi_519 into H_srtl_ynlohi1xvxvxhi1x_519.
+try rename h_sll_xnlohi1xvxvxhi1x_517 into h_sll_xnvxlo1xvxlo1xhi1xvxvxhi1x_517.
+try rename H_sll_xnlohi1xvxvxhi1x_517 into H_sll_xnvxlo1xvxlo1xhi1xvxvxhi1x_517.
+try rename h_sll_xnlohi1xvxvxhi1x_518 into h_sll_xnvxlo1xvxlo1xhi1xvxvxhi1x_518.
+try rename H_sll_xnlohi1xvxvxhi1x_518 into H_sll_xnvxlo1xvxlo1xhi1xvxvxhi1x_518.
+try rename h_srtl_ynlohi1xvxvxhi1x_519 into h_srtl_ynvxlo1xvxlo1xhi1xvxvxhi1x_519.
+try rename H_srtl_ynlohi1xvxvxhi1x_519 into H_srtl_ynvxlo1xvxlo1xhi1xvxvxhi1x_519.
+try rename h_srtl_ynvxlo1xvxlo1xhi1xvxvxhi1x_519 into h_srtl_ylen1xvxlo1xvxlo1xhi1xvxvxhi1x_519.
+try rename H_srtl_ynvxlo1xvxlo1xhi1xvxvxhi1x_519 into H_srtl_ylen1xvxlo1xvxlo1xhi1xvxvxhi1x_519.
+try rename h_sll_xnvxlo1xvxlo1xhi1xvxvxhi1x_518 into h_sll_xlen1xvxlo1xvxlo1xhi1xvxvxhi1x_518.
+try rename H_sll_xnvxlo1xvxlo1xhi1xvxvxhi1x_518 into H_sll_xlen1xvxlo1xvxlo1xhi1xvxvxhi1x_518.
+try rename h_sll_xnvxlo1xvxlo1xhi1xvxvxhi1x_517 into h_sll_xlen1xvxlo1xvxlo1xhi1xvxvxhi1x_517.
+try rename H_sll_xnvxlo1xvxlo1xhi1xvxvxhi1x_517 into H_sll_xlen1xvxlo1xvxlo1xhi1xvxvxhi1x_517.
+ssl_read x.
+try rename vx into vx2.
+try rename h_sll_xlen1xvxlo1xvxlo1xhi1xvxvxhi1x_518 into h_sll_xlen1xvx2lo1xvx2lo1xhi1xvx2vx2hi1x_518.
+try rename H_sll_xlen1xvxlo1xvxlo1xhi1xvxvxhi1x_518 into H_sll_xlen1xvx2lo1xvx2lo1xhi1xvx2vx2hi1x_518.
+try rename h_sll_xlen1xvxlo1xvxlo1xhi1xvxvxhi1x_517 into h_sll_xlen1xvx2lo1xvx2lo1xhi1xvx2vx2hi1x_517.
+try rename H_sll_xlen1xvxlo1xvxlo1xhi1xvxvxhi1x_517 into H_sll_xlen1xvx2lo1xvx2lo1xhi1xvx2vx2hi1x_517.
+try rename h_srtl_ylen1xvxlo1xvxlo1xhi1xvxvxhi1x_519 into h_srtl_ylen1xvx2lo1xvx2lo1xhi1xvx2vx2hi1x_519.
+try rename H_srtl_ylen1xvxlo1xvxlo1xhi1xvxvxhi1x_519 into H_srtl_ylen1xvx2lo1xvx2lo1xhi1xvx2vx2hi1x_519.
+ssl_read (x .+ 1).
+try rename nxtx into nxtx2.
+try rename h_sll_nxtxlen1xlo1xhi1x_513x into h_sll_nxtx2len1xlo1xhi1x_513x.
+try rename H_sll_nxtxlen1xlo1xhi1x_513x into H_sll_nxtx2len1xlo1xhi1x_513x.
+ssl_call_pre (r :-> null \+ h_sll_nxtx2len1xlo1xhi1x_513x).
+ssl_call (len1x, lo1x, hi1x).
+exists (h_sll_nxtx2len1xlo1xhi1x_513x);
+sslauto.
+move=>h_call0.
+ex_elim y1.
+ex_elim h_sll_nxtx2len1xlo1xhi1x_5181 h_srtl_y1len1xlo1xhi1x_5191.
+move=>[sigma_call0].
+subst h_call0.
+move=>[H_sll_nxtx2len1xlo1xhi1x_5181 H_srtl_y1len1xlo1xhi1x_5191].
+store_valid.
+ssl_read r.
+try rename y1 into y12.
+try rename h_srtl_y1len1xlo1xhi1x_5191 into h_srtl_y12len1xlo1xhi1x_5191.
+try rename H_srtl_y1len1xlo1xhi1x_5191 into H_srtl_y12len1xlo1xhi1x_5191.
+ssl_write r.
+ssl_call_pre (r :-> vx2 \+ h_srtl_y12len1xlo1xhi1x_5191).
+ssl_call (vx2, len1x, lo1x, hi1x).
+exists (h_srtl_y12len1xlo1xhi1x_5191);
+sslauto.
+move=>h_call1.
+ex_elim hi11 lo11 n11 y2.
+ex_elim h_srtl_y2n11lo11hi11_516.
+move=>[phi_call10] [phi_call11] [phi_call12].
+move=>[sigma_call1].
+subst h_call1.
+move=>H_srtl_y2n11lo11hi11_516.
+store_valid.
+try rename h_srtl_y2n11lo11hi11_516 into h_srtl_y2n11lo11hi1xvx2vx2hi1x_516.
+try rename H_srtl_y2n11lo11hi11_516 into H_srtl_y2n11lo11hi1xvx2vx2hi1x_516.
+try rename h_srtl_y2n11lo11hi1xvx2vx2hi1x_516 into h_srtl_y2n11vx2lo1xvx2lo1xhi1xvx2vx2hi1x_516.
+try rename H_srtl_y2n11lo11hi1xvx2vx2hi1x_516 into H_srtl_y2n11vx2lo1xvx2lo1xhi1xvx2vx2hi1x_516.
+try rename h_srtl_y2n11vx2lo1xvx2lo1xhi1xvx2vx2hi1x_516 into h_srtl_y2len1xvx2lo1xvx2lo1xhi1xvx2vx2hi1x_516.
+try rename H_srtl_y2n11vx2lo1xvx2lo1xhi1xvx2vx2hi1x_516 into H_srtl_y2len1xvx2lo1xvx2lo1xhi1xvx2vx2hi1x_516.
+ssl_read r.
+try rename y2 into y22.
+try rename h_srtl_y2len1xvx2lo1xvx2lo1xhi1xvx2vx2hi1x_516 into h_srtl_y22len1xvx2lo1xvx2lo1xhi1xvx2vx2hi1x_516.
+try rename H_srtl_y2len1xvx2lo1xvx2lo1xhi1xvx2vx2hi1x_516 into H_srtl_y22len1xvx2lo1xvx2lo1xhi1xvx2vx2hi1x_516.
+try rename h_srtl_ylen1xvx2lo1xvx2lo1xhi1xvx2vx2hi1x_519 into h_srtl_ylen1xvx2lo1xvx2lo1xhi1xvx2vx2hi1x_516.
+try rename H_srtl_ylen1xvx2lo1xvx2lo1xhi1xvx2vx2hi1x_519 into H_srtl_ylen1xvx2lo1xvx2lo1xhi1xvx2vx2hi1x_516.
+try rename h_srtl_ylen1xvx2lo1xvx2lo1xhi1xvx2vx2hi1x_516 into h_srtl_y22len1xvx2lo1xvx2lo1xhi1xvx2vx2hi1x_516.
+try rename H_srtl_ylen1xvx2lo1xvx2lo1xhi1xvx2vx2hi1x_516 into H_srtl_y22len1xvx2lo1xvx2lo1xhi1xvx2vx2hi1x_516.
+try rename h_sll_nxtx1len1x1lo12xhi12x_513x1 into h_sll_nxtx1len1x1lo12xhi12x_5181.
+try rename H_sll_nxtx1len1x1lo12xhi12x_513x1 into H_sll_nxtx1len1x1lo12xhi12x_5181.
+try rename h_sll_nxtx1len1x1lo12xhi12x_5181 into h_sll_nxtx1len1x1lo12xhi1x_5181.
+try rename H_sll_nxtx1len1x1lo12xhi12x_5181 into H_sll_nxtx1len1x1lo12xhi1x_5181.
+try rename h_sll_nxtx1len1x1lo12xhi1x_5181 into h_sll_nxtx1len1xlo12xhi1x_5181.
+try rename H_sll_nxtx1len1x1lo12xhi1x_5181 into H_sll_nxtx1len1xlo12xhi1x_5181.
+try rename h_sll_nxtx1len1xlo12xhi1x_5181 into h_sll_nxtx1len1xlo1xhi1x_5181.
+try rename H_sll_nxtx1len1xlo12xhi1x_5181 into H_sll_nxtx1len1xlo1xhi1x_5181.
+try rename h_sll_nxtx1len1xlo1xhi1x_5181 into h_sll_nxtx2len1xlo1xhi1x_5181.
+try rename H_sll_nxtx1len1xlo1xhi1x_5181 into H_sll_nxtx2len1xlo1xhi1x_5181.
+ssl_emp;
+exists (y22);
+exists (x :-> vx2 \+ x .+ 1 :-> nxtx2 \+ h_sll_nxtx2len1xlo1xhi1x_5181);
+exists (h_srtl_y22len1xvx2lo1xvx2lo1xhi1xvx2vx2hi1x_516);
+sslauto.
+unfold_constructor 2;
+exists (len1x), (vx2), (hi1x), (lo1x), (nxtx2), (h_sll_nxtx2len1xlo1xhi1x_5181);
+sslauto.
+Qed.
