examples/tree_flatten.v
@@ -1,0 +1,242 @@
+From mathcomp
+Require Import ssreflect ssrbool ssrnat eqtype seq ssrfun.
+From fcsl
+Require Import prelude pred pcm unionmap heap.
+From HTT
+Require Import stmod stsep stlog stlogR.
+From SSL
+Require Import core.
+
+Inductive tree (x : ptr) (s : seq nat) (h : heap) : Prop :=
+| tree_1 of x == null of
+  @perm_eq nat_eqType (s) (nil) /\ h = empty
+| tree_2 of (x == null) = false of
+  exists (v : nat) (s1 : seq nat) (s2 : seq nat) (l : ptr) (r : ptr),
+  exists h_tree_ls1_513 h_tree_rs2_514,
+  @perm_eq nat_eqType (s) ([:: v] ++ s1 ++ s2) /\ h = x :-> v \+ x .+ 1 :-> l \+ x .+ 2 :-> r \+ h_tree_ls1_513 \+ h_tree_rs2_514 /\ tree l s1 h_tree_ls1_513 /\ tree r s2 h_tree_rs2_514.
+
+Inductive treeN (x : ptr) (n : nat) (h : heap) : Prop :=
+| treeN_1 of x == null of
+  n == 0 /\ h = empty
+| treeN_2 of (x == null) = false of
+  exists (n1 : nat) (n2 : nat) (l : ptr) (r : ptr) (v : ptr),
+  exists h_treeN_ln1_515 h_treeN_rn2_516,
+  0 <= n1 /\ 0 <= n2 /\ n == 1 + n1 + n2 /\ h = x :-> v \+ x .+ 1 :-> l \+ x .+ 2 :-> r \+ h_treeN_ln1_515 \+ h_treeN_rn2_516 /\ treeN l n1 h_treeN_ln1_515 /\ treeN r n2 h_treeN_rn2_516.
+
+Inductive sll (x : ptr) (s : seq nat) (h : heap) : Prop :=
+| sll_1 of x == null of
+  @perm_eq nat_eqType (s) (nil) /\ h = empty
+| sll_2 of (x == null) = false of
+  exists (v : nat) (s1 : seq nat) (nxt : ptr),
+  exists h_sll_nxts1_517,
+  @perm_eq nat_eqType (s) ([:: v] ++ s1) /\ h = x :-> v \+ x .+ 1 :-> nxt \+ h_sll_nxts1_517 /\ sll nxt s1 h_sll_nxts1_517.
+
+Lemma tree_perm_eq_trans1 x h s_1 s_2 : perm_eq s_1 s_2 -> tree x s_1 h -> tree x s_2 h. Admitted.
+Hint Resolve tree_perm_eq_trans1: ssl_pred.
+Lemma sll_perm_eq_trans2 x h s_1 s_2 : perm_eq s_1 s_2 -> sll x s_1 h -> sll x s_2 h. Admitted.
+Hint Resolve sll_perm_eq_trans2: ssl_pred.
+Lemma pure3 : @perm_eq nat_eqType (nil) (nil). Admitted.
+Hint Resolve pure3: ssl_pure.
+Lemma pure4 vx22 s1x2 s2x2 : @perm_eq nat_eqType ([:: vx22] ++ s1x2 ++ s2x2) ([:: vx22] ++ s1x2 ++ s2x2). Admitted.
+Hint Resolve pure4: ssl_pure.
+
+Definition sll_append_type :=
+  forall (vprogs : ptr * ptr),
+  {(vghosts : seq nat * ptr * seq nat)},
+  STsep (
+    fun h =>
+      let: (x1, ret) := vprogs in
+      let: (s1, x2, s2) := vghosts in
+      exists h_sll_x1s1_518 h_sll_x2s2_519,
+      h = ret :-> x2 \+ h_sll_x1s1_518 \+ h_sll_x2s2_519 /\ sll x1 s1 h_sll_x1s1_518 /\ sll x2 s2 h_sll_x2s2_519,
+    [vfun (_: unit) h =>
+      let: (x1, ret) := vprogs in
+      let: (s1, x2, s2) := vghosts in
+      exists s y,
+      exists h_sll_ys_520,
+      @perm_eq nat_eqType (s) (s1 ++ s2) /\ h = ret :-> y \+ h_sll_ys_520 /\ sll y s h_sll_ys_520
+    ]).
+
+Variable sll_append : sll_append_type.
+
+Definition tree_flatten_type :=
+  forall (vprogs : ptr),
+  {(vghosts : ptr * seq nat)},
+  STsep (
+    fun h =>
+      let: (z) := vprogs in
+      let: (x, s) := vghosts in
+      exists h_tree_xs_521,
+      h = z :-> x \+ h_tree_xs_521 /\ tree x s h_tree_xs_521,
+    [vfun (_: unit) h =>
+      let: (z) := vprogs in
+      let: (x, s) := vghosts in
+      exists y,
+      exists h_sll_ys_522,
+      h = z :-> y \+ h_sll_ys_522 /\ sll y s h_sll_ys_522
+    ]).
+
+Program Definition tree_flatten : tree_flatten_type :=
+  Fix (fun (tree_flatten : tree_flatten_type) vprogs =>
+    let: (z) := vprogs in
+    Do (
+      x2 <-- @read ptr z;
+      if x2 == null
+      then
+        ret tt
+      else
+        vx22 <-- @read nat x2;
+        lx22 <-- @read ptr (x2 .+ 1);
+        rx22 <-- @read ptr (x2 .+ 2);
+        z ::= lx22;;
+        tree_flatten (z);;
+        y12 <-- @read ptr z;
+        z ::= rx22;;
+        tree_flatten (z);;
+        y22 <-- @read ptr z;
+        x2 ::= y22;;
+        sll_append (y12, x2);;
+        y32 <-- @read ptr x2;
+        y4 <-- allocb null 2;
+        dealloc x2;;
+        dealloc (x2 .+ 1);;
+        dealloc (x2 .+ 2);;
+        z ::= y4;;
+        (y4 .+ 1) ::= y32;;
+        y4 ::= vx22;;
+        ret tt
+    )).
+Obligation Tactic := intro; move=>z; ssl_program_simpl.
+Next Obligation.
+ssl_ghostelim_pre.
+move=>[x s].
+ex_elim h_tree_xs_521.
+move=>[sigma_self].
+subst h_self.
+move=>H_tree_xs_521.
+ssl_ghostelim_post.
+ssl_read z.
+try rename x into x2.
+try rename h_tree_xs_521 into h_tree_x2s_521.
+try rename H_tree_xs_521 into H_tree_x2s_521.
+ssl_open (x2 == null) H_tree_x2s_521.
+move=>[phi_tree_x2s_5210].
+move=>[sigma_tree_x2s_521].
+subst h_tree_x2s_521.
+shelve.
+ex_elim vx2 s1x2 s2x2 lx2 rx2.
+ex_elim h_tree_lx2s1x2_513x2 h_tree_rx2s2x2_514x2.
+move=>[phi_tree_x2s_5210].
+move=>[sigma_tree_x2s_521].
+subst h_tree_x2s_521.
+move=>[H_tree_lx2s1x2_513x2 H_tree_rx2s2x2_514x2].
+shelve.
+Unshelve.
+try rename h_sll_ys_522 into h_sll_y_522.
+try rename H_sll_ys_522 into H_sll_y_522.
+try rename h_tree_x2s_521 into h_tree_x2_521.
+try rename H_tree_x2s_521 into H_tree_x2_521.
+try rename h_sll_y_522 into h_sll__522.
+try rename H_sll_y_522 into H_sll__522.
+ssl_emp;
+exists (null);
+exists (empty);
+sslauto.
+unfold_constructor 1;
+sslauto.
+try rename h_sll_ys_522 into h_sll_yvx2s1x2s2x2_522.
+try rename H_sll_ys_522 into H_sll_yvx2s1x2s2x2_522.
+try rename h_tree_x2s_521 into h_tree_x2vx2s1x2s2x2_521.
+try rename H_tree_x2s_521 into H_tree_x2vx2s1x2s2x2_521.
+ssl_read x2.
+try rename vx2 into vx22.
+try rename h_sll_yvx2s1x2s2x2_522 into h_sll_yvx22s1x2s2x2_522.
+try rename H_sll_yvx2s1x2s2x2_522 into H_sll_yvx22s1x2s2x2_522.
+try rename h_tree_x2vx2s1x2s2x2_521 into h_tree_x2vx22s1x2s2x2_521.
+try rename H_tree_x2vx2s1x2s2x2_521 into H_tree_x2vx22s1x2s2x2_521.
+ssl_read (x2 .+ 1).
+try rename lx2 into lx22.
+try rename h_tree_lx2s1x2_513x2 into h_tree_lx22s1x2_513x2.
+try rename H_tree_lx2s1x2_513x2 into H_tree_lx22s1x2_513x2.
+ssl_read (x2 .+ 2).
+try rename rx2 into rx22.
+try rename h_tree_rx2s2x2_514x2 into h_tree_rx22s2x2_514x2.
+try rename H_tree_rx2s2x2_514x2 into H_tree_rx22s2x2_514x2.
+ssl_write z.
+ssl_call_pre (z :-> lx22 \+ h_tree_lx22s1x2_513x2).
+ssl_call (lx22, s1x2).
+exists (h_tree_lx22s1x2_513x2);
+sslauto.
+move=>h_call0.
+ex_elim y1.
+ex_elim h_sll_y1s1x2_5221.
+move=>[sigma_call0].
+subst h_call0.
+move=>H_sll_y1s1x2_5221.
+store_valid.
+ssl_read z.
+try rename y1 into y12.
+try rename h_sll_y1s1x2_5221 into h_sll_y12s1x2_5221.
+try rename H_sll_y1s1x2_5221 into H_sll_y12s1x2_5221.
+ssl_write z.
+ssl_call_pre (z :-> rx22 \+ h_tree_rx22s2x2_514x2).
+ssl_call (rx22, s2x2).
+exists (h_tree_rx22s2x2_514x2);
+sslauto.
+move=>h_call1.
+ex_elim y2.
+ex_elim h_sll_y2s2x2_5222.
+move=>[sigma_call1].
+subst h_call1.
+move=>H_sll_y2s2x2_5222.
+store_valid.
+ssl_read z.
+try rename y2 into y22.
+try rename h_sll_y2s2x2_5222 into h_sll_y22s2x2_5222.
+try rename H_sll_y2s2x2_5222 into H_sll_y22s2x2_5222.
+ssl_write x2.
+ssl_call_pre (x2 :-> y22 \+ h_sll_y12s1x2_5221 \+ h_sll_y22s2x2_5222).
+ssl_call (s1x2, y22, s2x2).
+exists (h_sll_y12s1x2_5221), (h_sll_y22s2x2_5222);
+sslauto.
+move=>h_call2.
+ex_elim s3 y3.
+ex_elim h_sll_y3s3_520.
+move=>[phi_call20].
+move=>[sigma_call2].
+subst h_call2.
+move=>H_sll_y3s3_520.
+store_valid.
+try rename h_sll_y3s3_520 into h_sll_y3s1x2s2x2_520.
+try rename H_sll_y3s3_520 into H_sll_y3s1x2s2x2_520.
+ssl_read x2.
+try rename y3 into y32.
+try rename h_sll_y3s1x2s2x2_520 into h_sll_y32s1x2s2x2_520.
+try rename H_sll_y3s1x2s2x2_520 into H_sll_y32s1x2s2x2_520.
+try rename h_sll_nxtys12y_517y into h_sll_nxtys12y_520.
+try rename H_sll_nxtys12y_517y into H_sll_nxtys12y_520.
+try rename h_sll_nxtys12y_520 into h_sll_y32s12y_520.
+try rename H_sll_nxtys12y_520 into H_sll_y32s12y_520.
+try rename h_sll_y32s12y_520 into h_sll_y32s1x2s2x2_520.
+try rename H_sll_y32s12y_520 into H_sll_y32s1x2s2x2_520.
+ssl_alloc y4.
+try rename y into y4.
+try rename h_sll_yvx22s1x2s2x2_522 into h_sll_y4vx22s1x2s2x2_522.
+try rename H_sll_yvx22s1x2s2x2_522 into H_sll_y4vx22s1x2s2x2_522.
+ssl_dealloc x2.
+ssl_dealloc (x2 .+ 1).
+ssl_dealloc (x2 .+ 2).
+ssl_write z.
+ssl_write_post z.
+ssl_write (y4 .+ 1).
+ssl_write_post (y4 .+ 1).
+ssl_write y4.
+ssl_write_post y4.
+ssl_emp;
+exists (y4);
+exists (y4 :-> vx22 \+ y4 .+ 1 :-> y32 \+ h_sll_y32s1x2s2x2_520);
+sslauto.
+unfold_constructor 2;
+exists (vx22), (s1x2 ++ s2x2), (y32), (h_sll_y32s1x2s2x2_520);
+sslauto.
+Qed.
